WIP; mem relation

security/BtInfoAsm.v
@@ -110,6 +110,46 @@ Section MEMDELTA.
       end.
   Proof. simpl. rewrite MEM. auto. Qed.
 
+  Definition mem_delta_apply_left (d: mem_delta) (om0: option mem) : option mem :=
+    fold_left (fun om data =>
+                 match data with
+                 | mem_delta_kind_store d => mem_delta_apply_store om d
+                 | mem_delta_kind_bytes d => mem_delta_apply_bytes om d
+                 | mem_delta_kind_alloc d => mem_delta_apply_alloc om d
+                 | mem_delta_kind_free d => mem_delta_apply_free om d
+                 end
+              ) d om0.
+
+  Lemma mem_delta_apply_left_cons
+        d m0 k
+    :
+    mem_delta_apply_left (k :: d) m0 =
+      match k with
+      | mem_delta_kind_store dd => mem_delta_apply_left d (mem_delta_apply_store (m0) dd)
+      | mem_delta_kind_bytes dd => mem_delta_apply_left d (mem_delta_apply_bytes (m0) dd)
+      | mem_delta_kind_alloc dd => mem_delta_apply_left d (mem_delta_apply_alloc (m0) dd)
+      | mem_delta_kind_free dd => mem_delta_apply_left d (mem_delta_apply_free (m0) dd)
+      end.
+  Proof. simpl. destruct k; auto. Qed.
+
+  Lemma mem_delta_apply_left_app
+        d0 d1 m0
+    :
+    mem_delta_apply_left (d0 ++ d1) m0 = mem_delta_apply_left d1 (mem_delta_apply_left d0 m0).
+  Proof.
+    revert d1 m0. induction d0; intros.
+    { simpl. auto. }
+    rewrite <- app_comm_cons. rewrite ! mem_delta_apply_left_cons. destruct a; auto.
+  Qed.
+
+  Lemma mem_delta_apply_eq
+        d m0
+    :
+    mem_delta_apply d m0 = mem_delta_apply_left (rev d) (Some m0).
+  Proof.
+    rewrite <- (rev_involutive d) at 1. unfold mem_delta_apply, mem_delta_apply_left. rewrite fold_left_rev_right. f_equal.
+  Qed.
+
   (* Delta and injection relation *)
   Definition mem_delta_kind_inj_wf (j: meminj): mem_delta_kind -> Prop :=
     fun data =>
@@ -122,20 +162,30 @@ Section MEMDELTA.
   Definition mem_delta_inj_wf (j: meminj): mem_delta -> Prop :=
     fun d => Forall (fun data => mem_delta_kind_inj_wf j data) d.
 
+  Lemma mem_delta_inj_wf_rev
+        j d
+    :
+    mem_delta_inj_wf j d <-> mem_delta_inj_wf j (rev d).
+  Proof.
+    unfold mem_delta_inj_wf. split; intros. apply Forall_rev; auto. rewrite <- rev_involutive. apply Forall_rev. auto.
+  Qed.
 
-  Definition mem_delta_inj_store_fo (j: meminj) (data: mem_delta_store): Prop :=
-    let '(ch, b, ofs, v, cp) := data in
-    match j b with
-    | Some _ => Forall (fun mv => match mv with | Byte bt => True | _ => False end) (encode_val ch v)
-    | None => True
-    end.
+  Definition meminj_first_order (j: meminj) (m: mem) :=
+    forall b ofs, (j b <> None) -> (Mem.perm m b ofs Cur Readable) -> loc_first_order m b ofs.
 
-  Definition mem_delta_inj_fo (j: meminj) (d: mem_delta): Prop :=
-    Forall (fun data =>
-              match data with
-              | mem_delta_kind_store d => mem_delta_inj_store_fo j d
-              | _ => True
-              end) d.
+  (* Definition mem_delta_inj_store_fo (j: meminj) (data: mem_delta_store): Prop := *)
+  (*   let '(ch, b, ofs, v, cp) := data in *)
+  (*   match j b with *)
+  (*   | Some _ => Forall (fun mv => match mv with | Byte bt => True | _ => False end) (encode_val ch v) *)
+  (*   | None => True *)
+  (*   end. *)
+
+  (* Definition mem_delta_inj_fo (j: meminj) (d: mem_delta): Prop := *)
+  (*   Forall (fun data => *)
+  (*             match data with *)
+  (*             | mem_delta_kind_store d => mem_delta_inj_store_fo j d *)
+  (*             | _ => True *)
+  (*             end) d. *)
 
   Definition mem_delta_apply_inj (j: meminj) (d: mem_delta) (m0: mem) : option mem :=
     fold_right (fun data om =>
@@ -149,6 +199,67 @@ Section MEMDELTA.
                   | _ => om
                   end) (Some m0) d.
 
+  Lemma mem_delta_apply_inj_cons
+        j d m0 m k
+        (MEM: mem_delta_apply_inj j d m0 = Some m)
+    :
+    mem_delta_apply_inj j (k :: d) m0 = 
+      match k with
+      | mem_delta_kind_store (ch, b, ofs, v, cp) =>
+          match j b with Some (b', ofsd) => mem_delta_apply_store (Some m) (ch, b', (ofs + ofsd)%Z, v, cp) | None => (Some m) end
+      | mem_delta_kind_bytes dd
+      | mem_delta_kind_alloc dd
+      | mem_delta_kind_free dd => Some m
+      end.
+  Proof. simpl. rewrite MEM. auto. Qed.
+
+  Definition mem_delta_apply_inj_left (j: meminj) (d: mem_delta) (om0: option mem) : option mem :=
+    fold_left (fun om data =>
+                 match data with
+                 | mem_delta_kind_store (ch, b, ofs, v, cp) =>
+                     match j b with
+                     | Some (b', ofsd) =>
+                         mem_delta_apply_store om (ch, b', (ofs + ofsd)%Z, v, cp)
+                     | None => om
+                     end
+                 | _ => om
+                 end) d (om0).
+
+  Lemma mem_delta_apply_inj_left_cons
+        j d m0 k
+    :
+    mem_delta_apply_inj_left j (k :: d) m0 =
+      match k with
+      | mem_delta_kind_store (ch, b, ofs, v, cp) =>
+          match j b with
+          | Some (b', ofsd) =>
+              mem_delta_apply_inj_left j d (mem_delta_apply_store m0 (ch, b', (ofs + ofsd)%Z, v, cp))
+          | None => mem_delta_apply_inj_left j d m0
+          end
+      | mem_delta_kind_bytes dd
+      | mem_delta_kind_alloc dd
+      | mem_delta_kind_free dd => mem_delta_apply_inj_left j d m0
+      end.
+  Proof. simpl. destruct k; auto. destruct d0 as [[[[a0 a1] a2] a3] a4]. destruct (j a1); auto. destruct p. auto. Qed.
+
+  Lemma mem_delta_apply_inj_left_app
+        j d0 d1 m0
+    :
+    mem_delta_apply_inj_left j (d0 ++ d1) m0 = mem_delta_apply_inj_left j d1 (mem_delta_apply_inj_left j d0 m0).
+  Proof.
+    revert j d1 m0. induction d0; intros.
+    { simpl. auto. }
+    rewrite <- app_comm_cons. rewrite ! mem_delta_apply_inj_left_cons. destruct a; auto.
+    { destruct d as [[[[a0 a1] a2] a3] a4]. destruct (j a1); auto. destruct p; auto. }
+  Qed.
+
+  Lemma mem_delta_apply_inj_eq
+        j d m0
+    :
+    mem_delta_apply_inj j d m0 = mem_delta_apply_inj_left j (rev d) (Some m0).
+  Proof.
+    rewrite <- (rev_involutive d) at 1. unfold mem_delta_apply_inj, mem_delta_apply_inj_left. rewrite fold_left_rev_right. f_equal.
+  Qed.
 
   Lemma alloc_left_unmapped_inject_keep:
     forall f m1 m2 c lo hi m1' b1,
@@ -212,6 +323,101 @@ Section MEMDELTA.
     intros; unfold f'; apply dec_eq_false; auto.
   Qed.
 
+  Lemma mem_delta_apply_preserves_full
+        (k j: meminj) m_i m0'
+        (INJ0: Mem.inject k m_i m0')
+        (INCR: inject_incr j k)
+        (d_pre d_post: mem_delta)
+        (DWFPRE: mem_delta_inj_wf j d_pre)
+        (DWFPOST: mem_delta_inj_wf j d_post)
+        m_m
+        (APPDPRE: mem_delta_apply_left d_pre (Some m_i) = Some m_m)
+        (WINJ: mem_weak_inject j m_m m0')
+        m_f
+        (APPDPOST: mem_delta_apply_left d_post (Some m_m) = Some m_f)
+        (MFO: meminj_first_order j m_f)
+    :
+    exists m1', (mem_delta_apply_inj j (d_pre ++ d_post) m0' = Some m1') /\ (Mem.inject j m_f m1').
+  Proof.
+
+
+
+    rewrite mem_delta_apply_eq in APPD. rewrite mem_delta_apply_inj_eq. rewrite mem_delta_inj_wf_rev in DWF. remember (rev d) as rd. clear d Heqrd. rename rd into d.
+    revert m0 m0' INJ0 DWF APPD. induction d; intros.
+    { unfold mem_delta_apply_inj_left. simpl. exists m0'. split; auto. unfold mem_delta_apply_left in APPD. simpl in APPD. inv APPD. auto. }
+    inv DWF. rename H1 into DWF1, H2 into DWF0.
+    rewrite mem_delta_apply_left_cons in APPD. rewrite mem_delta_apply_inj_left_cons.
+
+    
+
+
+    
+    revert DWF DFO m1 APPD. induction d; simpl; intros.
+    { inv APPD. exists m0'. split; auto. }
+    inv DWF. rename H1 into DWF1, H2 into DWF0. inv DFO. rename H1 into DFO1, H2 into DFO0.
+    destruct (mem_delta_apply d m0) eqn:DAM.
+    2:{ destruct a;
+        [rewrite mem_delta_apply_store_none in APPD; inv APPD
+        | rewrite mem_delta_apply_bytes_none in APPD; inv APPD
+        | rewrite mem_delta_apply_alloc_none in APPD; inv APPD
+        | rewrite mem_delta_apply_free_none in APPD; inv APPD].
+    }
+    rename m into m_i.
+    specialize (IHd DWF0 DFO0 _ (eq_refl)). destruct IHd as (m_i' & DAM' & INJ_I).
+    rewrite DAM'.
+    destruct a.
+    - destruct d0 as ((((ch & b) & ofs) & v) & cp). simpl in *.
+      destruct (j b) eqn:JB.
+      + destruct p as (b' & ofs'). eapply Mem.store_mapped_inject; eauto.
+        clear - DFO1. destruct v; auto. exfalso. simpl in *. destruct Archi.ptr64.
+        * destruct ch; simpl in *; try (inv DFO1; contradiction).
+        * destruct ch; simpl in *; try (inv DFO1; contradiction).
+      + exists m_i'; split; auto. eapply Mem.store_unmapped_inject; eauto.
+    - destruct d0 as (((b & ofs) & mvs) & cp). simpl in *.
+      exists m_i'; split; auto. eapply Mem.storebytes_unmapped_inject; eauto.
+    - destruct d0 as ((cp & lo) & hi). simpl in *.
+      exists m_i'; split; auto. destruct (Mem.alloc m_i cp lo hi) eqn:ALLOC. simpl in *. inv APPD.
+      eapply alloc_left_unmapped_inject_keep; eauto.
+    - destruct d0 as (((b & lo) & hi) & cp). simpl in *.
+      exists m_i'; split; auto. eapply Mem.free_left_inject; eauto.
+  Qed.
+
+  Lemma val_inject_incr_inv
+        f f' v v'
+        (INCR: inject_incr f f')
+        (INJ: Val.inject f' v v')
+    :
+    Val.inject f v v'.
+  Proof.
+    inv INJ; auto. eapply Val.inject_ptr; auto.
+val_inject_incr: forall (f1 f2 : meminj) (v v' : val), inject_incr f1 f2 -> Val.inject f1 v v' -> Val.inject f2 v v'
+
+  Lemma mem_inject_incr
+        f f' m m'
+        (INCR: inject_incr f f')
+        (INJ: Mem.inject f' m m')
+    :
+    Mem.inject f m m'.
+  Proof.
+    unfold Mem.inject in *. inv INJ. split; eauto.
+    2:{ intros. specialize (mi_freeblocks _ H). unfold inject_incr in INCR.
+        destruct (f b) eqn:FB; auto. destruct p. specialize (INCR _ _ _ FB).
+        rewrite INCR in mi_freeblocks. inv mi_freeblocks.
+    }
+    2:{ clear - INCR mi_no_overlap. unfold Mem.meminj_no_overlap in *. intros.
+        exploit mi_no_overlap; eauto.
+    }
+    clear - INCR mi_inj. inv mi_inj. split; eauto. intros. exploit mi_memval; eauto. intros.
+    eapply memval_inject_incr; eauto.
+    `
+    
+val_inject_incr: forall (f1 f2 : meminj) (v v' : val), inject_incr f1 f2 -> Val.inject f1 v v' -> Val.inject f2 v v'
+Unusedglobproof.regset_inject_incr: forall (f f' : meminj) (rs rs' : RTL.regset), Unusedglobproof.regset_inject f rs rs' -> inject_incr f f' -> Unusedglobproof.regset_inject f' rs rs'
+memval_inject_incr: forall (f f' : meminj) (v1 v2 : memval), memval_inject f v1 v2 -> inject_incr f f' -> memval_inject f' v1 v2
+Stackingproof.agree_regs_inject_incr: forall (j : meminj) (ls : Linear.locset) (rs : Mach.regset) (j' : meminj), Stackingproof.agree_regs j ls rs -> inject_incr j j' -> Stackingproof.agree_regs j' ls rs
+Cminorgenproof.match_temps_invariant: forall (f f' : meminj) (le : Csharpminor.temp_env) (te : Cminor.env), Cminorgenproof.match_temps f le te -> inject_incr f f' -> Cminorgenproof.match_temps f' le te
+val_inject_list_incr: forall (f1 f2 : meminj) (vl vl' : list val), inject_incr f1 f2 -> Val.inject_list f1 vl vl' -> Val.inject_list f2 vl vl'
+
   Lemma mem_delta_apply_preserves_inj
         (j: meminj) m0 m0'
         (INJ0: Mem.inject j m0 m0')
@@ -253,12 +459,118 @@ Section MEMDELTA.
       exists m_i'; split; auto. eapply Mem.free_left_inject; eauto.
   Qed.
 
+  Definition meminj_first_order (j: meminj) (m: mem) :=
+    forall b ofs, (j b <> None) -> (Mem.perm m b ofs Cur Readable) -> loc_first_order m b ofs.
+
+  Lemma mem_delta_apply_preserves_inj_incr
+        (j k: meminj) m0 m0'
+        (INCR: inject_incr j k)
+        (INJ0: Mem.inject k m0 m0')
+        (d: mem_delta)
+        (DWF: mem_delta_inj_wf j d)
+        (DFO: mem_delta_inj_fo j d)
+        m1
+        (APPD: mem_delta_apply d m0 = Some m1)
+        (MIFO: meminj_first_order j m1)
+    :
+    exists m1', (mem_delta_apply_inj j d m0' = Some m1') /\ (Mem.inject j m1 m1').
+  Proof.
+    revert DWF DFO m1 APPD MIFO. induction d; simpl; intros.
+    { inv APPD. exists m0'. split; auto. admit. (* MIFO *) }
+    inv DWF. rename H1 into DWF1, H2 into DWF0. inv DFO. rename H1 into DFO1, H2 into DFO0.
+    destruct (mem_delta_apply d m0) eqn:DAM.
+    2:{ destruct a;
+        [rewrite mem_delta_apply_store_none in APPD; inv APPD
+        | rewrite mem_delta_apply_bytes_none in APPD; inv APPD
+        | rewrite mem_delta_apply_alloc_none in APPD; inv APPD
+        | rewrite mem_delta_apply_free_none in APPD; inv APPD].
+    }
+    rename m into m_i.
+    specialize (IHd DWF0 DFO0 _ (eq_refl)). destruct IHd as (m_i' & DAM' & INJ_I).
+    { unfold meminj_first_order in *. intros. rename d into deltas.
+      specialize (MIFO _ ofs H). exploit MIFO; clear MIFO.
+      { destruct a; simpl in *.
+        - unfold mem_delta_apply_store in APPD. destruct d as [[[[ch0 b0] ofs0] v0] cp0].
+          eapply Mem.perm_store_1; eauto.
+        - unfold mem_delta_apply_bytes in APPD. destruct d as [[[b0 ofs0] mvs0] cp0].
+          eapply Mem.perm_storebytes_1; eauto.
+        - unfold mem_delta_apply_alloc in APPD. destruct d as [[cp0 lo0] hi0].
+          destruct (Mem.alloc m_i cp0 lo0 hi0) eqn:CASES. inv APPD.
+          eapply Mem.perm_alloc_1; eauto. 
+        - unfold mem_delta_apply_free in APPD. destruct d as [[[b0 lo0] hi0] cp0].
+          eapply Mem.perm_free_1; eauto. left. intros EQ. subst. rewrite DWF1 in H. congruence.
+      }
+      intros MIFO. clear H0.
+      { destruct a; simpl in *.
+        - unfold mem_delta_apply_store in APPD. destruct d as [[[[ch0 b0] ofs0] v0] cp0].
+          destruct (Pos.eqb_spec b b0).
+          + subst b0. unfold mem_delta_inj_store_fo in DFO1.
+            destruct (j b) eqn:JB. 2: congruence. clear H. destruct p.
+            unfold loc_first_order in *. clear MIFO APPD.
+            
+
+            
+Mem.store_mem_contents:
+  forall (chunk : memory_chunk) (m1 : mem) (b : block) (ofs : Z) (v : val) 
+    (cp : compartment) (m2 : mem),
+  Mem.store chunk m1 b ofs v cp = Some m2 ->
+  Mem.mem_contents m2 =
+  PMap.set b (Mem.setN (encode_val chunk v) ofs (Mem.mem_contents m1) !! b) (Mem.mem_contents m1)
+
+
+          
+          eapply Mem.perm_store_1; eauto.
+        - unfold mem_delta_apply_bytes in APPD. destruct d as [[[b0 ofs0] mvs0] cp0].
+          eapply Mem.perm_storebytes_1; eauto.
+        - unfold mem_delta_apply_alloc in APPD. destruct d as [[cp0 lo0] hi0].
+          destruct (Mem.alloc m_i cp0 lo0 hi0) eqn:CASES. inv APPD.
+          eapply Mem.perm_alloc_1; eauto. 
+        - unfold mem_delta_apply_free in APPD. destruct d as [[[b0 lo0] hi0] cp0].
+          eapply Mem.perm_free_1; eauto. left. intros EQ. subst. rewrite DWF1 in H. congruence.
+      }
+
+
+
+      
+    rewrite DAM'.
+    destruct a.
+    - destruct d0 as ((((ch & b) & ofs) & v) & cp). simpl in *.
+      destruct (j b) eqn:JB.
+      + destruct p as (b' & ofs'). eapply Mem.store_mapped_inject; eauto.
+        clear - DFO1. destruct v; auto. exfalso. simpl in *. destruct Archi.ptr64.
+        * destruct ch; simpl in *; try (inv DFO1; contradiction).
+        * destruct ch; simpl in *; try (inv DFO1; contradiction).
+      + exists m_i'; split; auto. eapply Mem.store_unmapped_inject; eauto.
+    - destruct d0 as (((b & ofs) & mvs) & cp). simpl in *.
+      exists m_i'; split; auto. eapply Mem.storebytes_unmapped_inject; eauto.
+    - destruct d0 as ((cp & lo) & hi). simpl in *.
+      exists m_i'; split; auto. destruct (Mem.alloc m_i cp lo hi) eqn:ALLOC. simpl in *. inv APPD.
+      eapply alloc_left_unmapped_inject_keep; eauto.
+    - destruct d0 as (((b & lo) & hi) & cp). simpl in *.
+      exists m_i'; split; auto. eapply Mem.free_left_inject; eauto.
+  Qed.
+
   (* Memory injection for public global symbols: visible for external calls *)
   Definition meminj_public (ge: Senv.t): meminj :=
     fun b => match Senv.invert_symbol ge b with
           | Some id => if Senv.public_symbol ge id then Some (b, 0%Z) else None
           | None => None
           end.
+
+
+        (DFO: mem_delta_inj_fo j d)
+                            visible_fo_if_unknown ef ge m vargs ->
+    | None => visible_fo ge m (sig_args sg) args
+visible_fo =
+fun (ge : Senv.t) (m : mem) (tys : list typ) (args : list val) =>
+public_first_order ge m /\ vals_public ge tys args
+     : Senv.t -> mem -> list typ -> list val -> Prop
+public_first_order =
+fun (ge : Senv.t) (m : mem) =>
+forall (id : ident) (b : block) (ofs : Z),
+Senv.public_symbol ge id = true ->
+Senv.find_symbol ge id = Some b -> Mem.perm m b ofs Cur Readable -> loc_first_order m b ofs
+     : Senv.t -> mem -> Prop
 
   (* TODO: this is false --- pointers can mess around *)
 (*   Lemma val_inject_incr_inv *)
@@ -279,9 +591,16 @@ Section MEMDELTA.
     Mem.inject f m m'.
   Proof.
     unfold Mem.inject in *. inv INJ. split; eauto.
-    - clear - INCR mi_inj. inv mi_inj. split; eauto. intros. exploit mi_memval; eauto. intros.
-      eapply memval_inject_incr; eauto.
-    
+    2:{ intros. specialize (mi_freeblocks _ H). unfold inject_incr in INCR.
+        destruct (f b) eqn:FB; auto. destruct p. specialize (INCR _ _ _ FB).
+        rewrite INCR in mi_freeblocks. inv mi_freeblocks.
+    }
+    2:{ clear - INCR mi_no_overlap. unfold Mem.meminj_no_overlap in *. intros.
+        exploit mi_no_overlap; eauto.
+    }
+    clear - INCR mi_inj. inv mi_inj. split; eauto. intros. exploit mi_memval; eauto. intros.
+    eapply memval_inject_incr; eauto.
+    `
     
 val_inject_incr: forall (f1 f2 : meminj) (v v' : val), inject_incr f1 f2 -> Val.inject f1 v v' -> Val.inject f2 v v'
 Unusedglobproof.regset_inject_incr: forall (f f' : meminj) (rs rs' : RTL.regset), Unusedglobproof.regset_inject f rs rs' -> inject_incr f f' -> Unusedglobproof.regset_inject f' rs rs'
